solvers/49.lean
@@ -3,4 +3,4 @@ import ProjectEulerSolutions.P49
 open ProjectEulerSolutions.P49
 
 def main : IO Unit := do
-  IO.println (serialize (solve 10000))
+  IO.println (serialize (solve 4 3))
